src/named/SimpleVCPS.v
@@ -212,11 +212,12 @@ Lemma term_con_congruence l c t name s1 s2 c' args t'
   : In (name, term_rule c' args t') l ->
     len_eq c' s2 ->
     t = t'[/with_names_from c' s2/] ->
-    wf_ctx l c' ->
+    wf_lang l ->
     eq_args l c c' s1 s2 ->
     eq_term l c t (con name s1) (con name s2).
 Proof.
   intros.
+  assert (wf_ctx l c') by with_rule_in_wf_crush.
   rewrite <- (wf_con_id_args_subst c' s1);[| basic_core_crush..].
   rewrite <- (wf_con_id_args_subst c' s2);[|basic_core_crush..].
   subst.
@@ -229,7 +230,91 @@ Proof.
   basic_core_crush.
 Qed.
 
-Axiom TODO: False.
+(*TDO: move to matches or new parstep file*)
+(*If the LHS of a term eq rule directly applies to e, 
+  return the rule name and s such that LHS[/s/] = e.
+  Rules are scanned from the root of the language.
+ *)
+Import OptionMonad.
+
+Inductive step_instruction :=
+| cong_instr : list step_instruction -> step_instruction
+| refl_instr : step_instruction
+| redex_instr : string -> ctx -> sort -> exp -> exp -> subst -> step_instruction.
+
+Fixpoint step_redex_term (l : lang) (e : exp) : option step_instruction :=
+  match l with
+  | [] => None
+  | (n,term_eq_rule c e1 e2 t')::l' =>
+    match step_redex_term l' e with
+    | Some e' => Some e'
+    | None => do s <- matches e e1 (map fst c);
+              ret (redex_instr n c t' e1 e2 s)
+    end
+  | _::l' => step_redex_term l' e
+  end.
+
+(*TODO: move to Utils.OptionMonad*)
+Section Mmap.
+  Context  {A B} (f : A -> option B).
+  Fixpoint Mmap (l_a : list A) : option (list B) :=
+    match l_a with
+    | [] => do ret []
+             | a::l_a' =>
+               do l_b' <- Mmap l_a';
+               b <- f a;
+            ret (b::l_b')
+    end.
+End Mmap.
+
+Fixpoint step_term l e : option step_instruction :=
+  match step_redex_term l e with
+  | Some i => Some i
+  | None =>
+    match e with
+    | var x => Some refl_instr
+    | con n s =>
+      option_map cong_instr (Mmap (step_term l) s)
+    end
+  end.
+
+
+Require Import Ltac2.Ltac2.
+Import Ltac2.Message Ltac2.Control.
+Set Default Proof Mode "Classic".
+
+Lemma wf_args_cons2
+     : forall (l : lang) (c : ctx) (s : list exp) (c' : named_list sort) 
+         (name name': string) (e e': exp) (t t' : sort),
+       wf_term l c e' t' [/with_names_from ((name,t)::c') (e::s) /] ->
+       wf_term l c e t [/with_names_from c' s /] ->
+       wf_args l c s c' -> wf_args l c (e'::e :: s) ((name',t')::(name, t) :: c').
+Proof.
+  eauto with lang_core.
+Qed.
+
+Lemma eq_args_cons2
+     : forall (l : lang) (c : ctx) (s1 s2 : list exp) (c' : named_list sort) 
+         (name name': string) (e1 e2 e1' e2': exp) (t t' : sort),
+       eq_term l c t' [/with_names_from ((name,t)::c') (e2::s2) /] e1' e2'->
+       eq_term l c t [/with_names_from c' s2 /] e1 e2 ->
+       eq_args l c c' s1 s2 ->
+       eq_args l c ((name',t')::(name, t) :: c') (e1'::e1 :: s1) (e2'::e2 :: s2) .
+Proof.
+  eauto with lang_core.
+Qed.
+
+Lemma eq_term_by_with_subst name l c c' e1 e2 t s 
+  : wf_lang l ->
+    In (name, term_eq_rule c' e1 e2 t) l ->
+    wf_subst l c s c' ->
+    eq_term l c t[/s/] e1[/s/] e2[/s/].
+Proof.
+  intros.
+  eapply eq_term_subst; [| eapply eq_subst_refl; eassumption
+                         | eapply eq_term_by; eassumption].
+  with_rule_in_wf_crush.
+Qed.
   
 Derive cps_elab
        SuchThat (elab_preserving_compiler stlc_bot_elab comp cps_elab stlc_elab)
@@ -283,22 +368,32 @@ Proof.
      change (eq_term l ctx' e1' e2' t')
     end.
 
+
+  Ltac solve_in := apply named_list_lookup_err_in; compute; reflexivity.
+
+  Ltac lookup_wf_lang := admit (*TODO: add to ctx beforehand, use assumption here*).
   
+(*TODO: optimize where this is used so that I don't
+  duplicate work?
+*)
 Local Ltac t' :=
   match goal with
   | [|- fresh _ _ ]=> apply use_compute_fresh; compute; reflexivity
   | [|- sublist _ _ ]=> apply (use_compute_sublist string_dec); compute; reflexivity
-  | [|- In _ _ ]=> apply named_list_lookup_err_in; compute; reflexivity
-  | [|- wf_term _ _ _ _] =>  eapply wf_term_var || eapply wf_term_by'
-  | [|-wf_args _ _ _ _] => econstructor
-  | [|-wf_subst _ _ _ _] => econstructor
-  | [|-wf_ctx _ _] => econstructor
+  | [|- In _ _ ]=> solve_in
+  | [|- wf_term _ _ _ _] => assumption || eapply wf_term_var || eapply wf_term_by'
+  | [|-wf_args _ _ _ _] => simple apply wf_args_nil
+                           || simple eapply wf_args_cons2
+                           || simple eapply wf_args_cons
+  | [|-wf_subst _ _ _ _] => constructor
+  | [|-wf_ctx _ _] => assumption || constructor
   | [|- wf_sort _ _ _] => eapply wf_sort_by
+  | [|- wf_lang _] => lookup_wf_lang
   | [|- _ = _] => compute; reflexivity
   end.
 
 Ltac eq_term_by s := 
-  eapply (eq_term_by _ _ s); solve[repeat t'].
+  eapply (eq_term_by _ _ s); solve_in.
 
 (*TODO: adapt to work w/ possible evars in r?*)
 Ltac solve_named_list_in_from_value :=
@@ -314,17 +409,23 @@ Ltac solve_named_list_in_from_value :=
 
 Ltac is_term_rule := eapply eq_term_by; solve_named_list_in_from_value.
 
-    Ltac term_cong :=
+Ltac solve_len_eq := solve[ repeat constructor].
+
+Ltac term_cong :=
       eapply term_con_congruence;
-      [t'
-      | solve[ repeat constructor]
+      [ solve_in
+      | solve_len_eq
       | compute; reflexivity
-      |try solve [repeat t']
+      | lookup_wf_lang
       | repeat match goal with [|- eq_args _ _ _ _ _] =>
-                              constructor
+                               constructor
+               (*
+                simple apply eq_args_nil
+                           || simple eapply eq_args_cons2
+                           || simple eapply eq_args_cons*)
                end].
     Ltac term_refl := 
-      apply eq_term_refl; solve[repeat t'].
+      apply eq_term_refl; admit (*TODO: solve[repeat t']*).
     
     (*TODO: only works if all variables appear on the lhs*)
     Ltac redex_steps_with name :=
@@ -349,30 +450,240 @@ Ltac is_term_rule := eapply eq_term_by; solve_named_list_in_from_value.
     | _ => fail "Rule not found"
     end.
 
-    
-    Ltac redex_steps_from_list l :=
-      lazymatch l with
-      | ?n :: ?l' =>
-        redex_steps_with n || (redex_steps_from_list l')
-      | _ => fail "No redex found"
+    Ltac2 step_redex name c' tp e1p e2p s :=
+        lazy_match! goal with
+        | [|- eq_term ?l ?c _ _ _] =>
+          assert (eq_term $l $c $tp[/$s/] $e1p[/$s/] $e2p[/$s/])> [| ltac1:(eassumption)];
+          apply (@eq_term_by_with_subst $name $l $c $c' $e1p $e2p $tp $s); solve [repeat ltac1:(t')]
+          (*
+          eapply (@eq_term_subst $l $c $s $s $c')>
+          [repeat ltac1:(t'); shelve()
+          | eapply eq_subst_refl; repeat ltac1:(t'); shelve()
+          | eapply (@eq_term_by $l $c' $name); repeat ltac1:(t'); shelve()]
+*)
+        end.
+(*      lazy_match! goal with
+      | [|- eq_term ?l ?c' ?t ?e1 ?e2] =>
+        let ms := Std.eval_vm None constr:(matches $e1 $e1p (map fst $c)) in
+            lazy_match! ms with
+            | Some ?s =>
+              assert (eq_term $l $c' $tp[/$s/] $e1p[/$s/] $e2p[/$s/])> [| assumption]
+            | None => backtrack_tactic_failure "lhs does not match rule"
+            end
+      | [|-_] => backtrack_tactic_failure "Goal not a term equality"
+      end.
+*)
+(*
+  
+                [| reflexivity];
+                eapply eq_term_subst;
+                [| | eq_term_by name];
+                [solve [repeat t']|apply eq_subst_refl; solve [repeat t']]
+ *)
+    Ltac2 get_goal_lang () :=
+      lazy_match! goal with
+      |[|- eq_term ?l _ _ _ _ ] => l
       end.
 
-    Ltac rstp := let rnames := eval compute in (map fst stlc_bot_elab) in
-                     redex_steps_from_list rnames.
+    Ltac2 rec step_by_instructions i :=
+      lazy_match! i with
+      | refl_instr => ltac1:(term_refl)
+      | cong_instr ?s =>
+        (*have to run this before term_cong because for some reason
+          it expects a focussed goal
+         *)
+        let s_tac_list := List.rev (step_all_instructions s) in
+        ltac1:(term_cong);
+        Control.dispatch s_tac_list
+      | redex_instr ?name ?c' ?tp ?e1p ?e2p ?s =>
+        step_redex name c' tp e1p e2p s
+      | _ => backtrack_tactic_failure "input not an evaluated instruction"
+    end
+    with step_all_instructions s :=
+      lazy_match! s with
+      | [] => []
+      | ?i::?s' => (fun () => step_by_instructions i)::(step_all_instructions s')
+      | _ => backtrack_tactic_failure "input not an evaluated list"
+      end.
+
+    Ltac2 get_step_instructions () :=
+    lazy_match! goal with
+     | [|- eq_term ?l ?c' ?t ?e1 ?e2] =>
+       let mi := Std.eval_vm None constr:(step_term $l $e1) in
+       lazy_match! mi with
+       | Some ?i => i
+       | None =>  backtrack_tactic_failure "could not generate step instructions"
+       end
+     | [|-_] => backtrack_tactic_failure "goal not a term equality"
+  end.
+      
+    Ltac2 step () :=
+      step_by_instructions (get_step_instructions ()).
+  
+    Ltac par_step :=
+      lazymatch goal with
+        [|- eq_term ?l ?c ?t ?e1 ?e2] =>
+        let mns := eval compute in (step_term l e1) in
+            lazymatch mns with
+            | Some (redex_instr ?name ?c' ?tp ?e1p ?e2p ?s) =>
+              replace (eq_term l c t e1 e2)
+                with (eq_term l c tp[/s/] e1p[/s/] e2p[/s/]);
+                [| reflexivity];
+                apply (@eq_term_subst l c s s c' tp e1p e2p);
+                [solve [repeat t']| | eq_term_by name];[];
+                apply eq_subst_refl; solve [repeat t']             
+            | None => fail "No redex found"
+            end
+      | _ => fail "Goal not a term equality"
+      end.
     
+    Ltac redex_step :=
+      lazymatch goal with
+        [|- eq_term ?l ?c ?t ?e1 ?e2] =>
+        let mns := eval compute in (step_redex_term l e1) in
+            lazymatch mns with
+            | Some (redex_instr ?name ?c' ?tp ?e1p ?e2p ?s) =>
+              replace (eq_term l c t e1 e2)
+                with (eq_term l c tp[/s/] e1p[/s/] e2p[/s/]);
+                [| reflexivity];
+                apply (@eq_term_subst l c s s c' tp e1p e2p);
+                [solve [repeat t']| | eq_term_by name];[];
+                apply eq_subst_refl; solve [repeat t']             
+            | None => fail "No redex found"
+            end
+      | _ => fail "Goal not a term equality"
+      end.
+    
+    (*TODO: Coq fn that does this computation
+      TODO: what should that fn return?
+     *)
     Ltac one_par_step :=
-      rstp || (term_cong; one_par_step) || term_refl.
-    Ltac reduce := repeat (eapply eq_term_trans; [one_par_step|compute_eq_compilation]).
+      redex_step || (term_cong; one_par_step) || term_refl.
+    Ltac reduce := repeat (progress (eapply eq_term_trans; [ltac2:(step())|])); term_refl.
     Ltac by_reduction :=
-      eapply eq_term_trans; [reduce; term_refl | eapply eq_term_sym; reduce; term_refl].
+      eapply eq_term_trans; [reduce | eapply eq_term_sym; reduce].
   
 auto_elab_compiler; compute_eq_compilation.
 all: try solve [is_term_rule].
- by_reduction.
- by_reduction.
- by_reduction.
- 3: by_reduction.
- (*TODO: too slow to run on remaining 2 *)
+
+Set Ltac Profiling.
+solve[by_reduction].
+solve[by_reduction].
+solve[by_reduction].
+Show Ltac Profile.
+(*solve[by_reduction].
+solve[by_reduction].
+3:solve[by_reduction].*)
+(*TODO: haven't solved the perf. issues; do some analysis*)
+3:{
+  eapply eq_term_trans.
+  {
+    Set Ltac Profiling.
+    (*TODO: how to make sure I only assert things
+      about intermediate contexts once?
+      alt: use rule_in_wf?
+      better lemmas?
+     *)
+    time (progress (eapply eq_term_trans;[ltac2:(step())|])).
+    Show Ltac Profile.
+
+    progress (eapply eq_term_trans;[ltac2:(step())|]).
+    progress (eapply eq_term_trans;[ltac2:(step())|]).
+    progress (eapply eq_term_trans;[ltac2:(step())|]).
+    compute_eq_compilation.
+    progress (eapply eq_term_trans;[ltac2:(step())|]).
+    progress (eapply eq_term_trans;[ltac2:(step())|]).
+  term_refl.
+}
+    ltac2:(step()).
+    {
+      compute_eq_compilation.
+      term_cong.
+      ltac2:(step()).
+      ltac2:(step()).
+      ltac2:(step()).
+      {
+        ltac2:(step()).
+        eapply eq_term_subst.
+        compute_eq_compilation.
+        2:{
+          cbn in H.
+          compute_eq_compilation.
+          exact H.
+        ltac2:(let i := (get_step_instructions()) in
+               lazy_match! i with
+               | redex_instr ?name ?c' ?tp ?e1p ?e2p ?s =>
+                 step_redex name c' tp e1p e2p s; solve []
+               | _ => backtrack_tactic_failure "input not an evaluated instruction"
+               end
+              ).
+        Definition ctxid (c:ctx) := c.
+        ltac2:(step_redex
+                 constr:("id_right")
+                 constr:(ctxid {{c"G" : #"env", "G'" : #"env", "f" : # "sub" %"G" %"G'"}})
+                 constr:({{s# "sub" %"G" %"G'"}})
+                          constr:({{e# "cmp" %"G" %"G'" %"G'" %"f" (# "id" %"G'")}})
+                                   constr:({{e%"f"}})
+                 constr:([("f", {{e# "wkn" %"G" (# "->" %"A" #"bot")}}); ("G'", {{e%"G"}});
+   ("G", {{e# "ext" %"G" (# "->" %"A" #"bot")}})])).
+      ltac2:(step()).
+    
+    {
+      ltac2:(print (of_constr (get_step_instructions()) )).
+    
+      ltac2:(step()).
+      
+    ltac2:(lazy_match! goal with
+     | [|- eq_term ?l ?c' ?t ?e1 ?e2] =>
+       let mi := Std.eval_vm None constr:(step_term $l $e1) in
+       lazy_match! mi with
+       | Some ?i => print (of_constr i)
+       | None =>  backtrack_tactic_failure "could not generate step instructions"
+       end
+     | [|-_] => backtrack_tactic_failure "goal not a term equality"
+  end).
+      ltac2:(step()).
+    (*TODO: understand what isn't focussed and why*)
+    term_cong;
+      ltac2:(dispatch [
+                 (fun () => try ltac1:(term_refl));
+                 (fun () => try ltac1:(term_refl));
+                 (fun () => try ltac1:(term_refl));
+                 (fun () => try ltac1:(term_refl));
+                 (fun () => try ltac1:(term_refl))]).                 
+  }
+  
+  term_cong.
+  term_refl.
+  {
+    compute_eq_compilation.
+    term_cong.
+    term_refl.
+    
+
+  term_cong;
+    [term_refl
+    | term_cong; solve[fail]
+    | term_cong;
+      [ term_cong; [term_cong; [term_cong; solve[fail]| term_refl] | term_refl]
+      | (*TODO*)
+      | term_cong; [term
+    ]].
+  (cong_instr
+   [refl_instr; cong_instr [];
+   cong_instr
+     [cong_instr [cong_instr [cong_instr []; refl_instr]; refl_instr];
+     redex_instr "id_right" {{c"G" : #"env", "G'" : #"env", "f" : # "sub" %"G" %"G'"}} {{s# "sub" %"G" %"G'"}}
+       {{e# "cmp" %"G" %"G'" %"G'" %"f" (# "id" %"G'")}} {{e%"f"}}
+       [("f", {{e# "wkn" %"G" (# "->" %"A" #"bot")}}); ("G'", {{e%"G"}}); ("G", {{e# "ext" %"G" (# "->" %"A" #"bot")}})];
+     cong_instr [cong_instr []; refl_instr]; refl_instr; cong_instr [cong_instr [cong_instr []; refl_instr]; refl_instr]];
+   cong_instr [cong_instr [cong_instr []; refl_instr]; refl_instr]; cong_instr [cong_instr [cong_instr []; refl_instr]; refl_instr]])
+by_reduction.
+by_reduction.
+by_reduction.
+3: by_reduction.
+by_reduction.
+ (*TODO: too slow to run on remaining 2*)
  destruct TODO.
  destruct TODO.
  Unshelve.
